inst type henry ford encode

Translation/Ty.lean
@@ -7,18 +7,20 @@ import Surface.Typing
 import LeanSubst
 open LeanSubst
 
+namespace Surface
+
 @[simp]
-def Surface.Kind.translate : Surface.Kind -> Core.Kind
+def Kind.translate : Surface.Kind -> Core.Kind
 | .base .closed => .base .closed
 | .base .open => .base .open
 | .arrow k1 k2 => .arrow (translate k1) (translate k2)
 notation "⟦" K "⟧" => Surface.Kind.translate K
 
-def Surface.KindEnv.translate : Surface.KindEnv -> Core.KindEnv := List.map (·.translate)
+def KindEnv.translate : Surface.KindEnv -> Core.KindEnv := List.map (·.translate)
 notation "⟦" Δ "⟧" => Surface.KindEnv.translate Δ
 
 @[simp]
-def Surface.Ty.translate: Surface.Ty -> Core.Ty
+def Ty.translate: Surface.Ty -> Core.Ty
 | .var x => .var x
 | .global x => .global x
 | .arrow a b => .arrow (a.translate) (b.translate)
@@ -29,13 +31,59 @@ def Surface.Ty.translate: Surface.Ty -> Core.Ty
 notation "⟦" A "⟧" => Surface.Ty.translate A
 
 @[simp]
-def Surface.TyEnv.translate (Γ : TyEnv) : (List Core.Ty) :=
+def TyEnv.translate (Γ : TyEnv) : (List Core.Ty) :=
   Γ.map (·.translate)
 notation "⟦" Γ "⟧" => Surface.TyEnv.translate Γ
 
 @[simp]
-def Subst.Surface.Ty.translate (σ : Subst Surface.Ty) : Subst Core.Ty :=
+def Subst.Ty.translate (σ : Subst Surface.Ty) : Subst Core.Ty :=
   (λ x => match x with
   | .re x => .re x
   | .su T => .su (T.translate)) <$> σ
 notation "⟦" σ "⟧" => Subst.Surface.Ty.translate σ
+
+end Surface
+
+namespace Core
+
+@[simp]
+def Ty.fresh_vars : Nat -> List Nat
+| 0 => []
+| n + 1 => n :: fresh_vars n
+
+@[simp]
+def Ty.mk_arrow (b : Ty) : List Ty -> Ty
+| [] => b
+| .cons x xs => x -:> Ty.mk_arrow b xs
+
+@[simp]
+def Ty.mk_all (b : Ty) : Nat -> Ty
+| 0 => b
+| n + 1 => ∀[★] (Ty.mk_all b n)
+
+--- C τ1 τ2 ---> ∀ ∀ (1 ~ τ1) (0 ~ τ2)  -> C 0 1
+--- but also
+--- ∀αs. T βs => C τs ------> ∀
+@[simp]
+def Ty.InstEncode (τ : Ty) : Option Ty :=
+  match τ.spine with
+  | .some (x , sp) =>
+    let fvs := fresh_vars sp.length
+    let prefix_τs := (fvs.zip sp).map (λ (n, τ) => t#n ~[★]~ τ )
+    return ((((gt#x).apply (fvs.map (t#·))).mk_arrow prefix_τs).mk_all fvs.length)
+  | _ => none
+
+#eval Ty.InstEncode ((gt#"C").apply [gt#"a", gt#"b"] )
+
+
+
+theorem Ty.InstEncodeKindSound :
+  G&Δ ⊢ τ : ◯ ->
+  some τ' = Ty.InstEncode τ  ->
+  G&Δ ⊢ τ' : ◯ := by
+intro h1 h2
+induction τ <;> simp [Ty.spine, Ty.apply] at *
+case global => subst h2; apply h1
+case app => sorry
+
+end Core
